template-coq/theories/Ast.v
@@ -1,5 +1,6 @@
 (* Distributed under the terms of the MIT license.   *)
 
+Require Int63.
 Require Import Coq.Strings.String.
 Require Import Coq.PArith.BinPos.
 Require Import List. Import ListNotations.
@@ -59,7 +60,11 @@ Inductive term : Set :=
         (discr:term) (branches : list (nat * term))
 | tProj (proj : projection) (t : term)
 | tFix (mfix : mfixpoint term) (idx : nat)
-| tCoFix (mfix : mfixpoint term) (idx : nat).
+| tCoFix (mfix : mfixpoint term) (idx : nat)
+| tInt (i : Int63.int).
+
+(** Primitive integers type, as defined in the standard library. *)
+Definition tInt_type := tConst "Coq.Numbers.Cyclic.Int63.Int63.int"%string [].
 
 Definition mkApps t us :=
   match us with
@@ -104,7 +109,8 @@ Inductive wf : term -> Prop :=
 | wf_tProj p t : wf t -> wf (tProj p t)
 | wf_tFix mfix k : Forall (fun def => wf def.(dtype) /\ wf def.(dbody) /\ isLambda def.(dbody) = true) mfix ->
                    wf (tFix mfix k)
-| wf_tCoFix mfix k : Forall (fun def => wf def.(dtype) /\ wf def.(dbody)) mfix -> wf (tCoFix mfix k).
+| wf_tCoFix mfix k : Forall (fun def => wf def.(dtype) /\ wf def.(dbody)) mfix -> wf (tCoFix mfix k)
+| wf_tInt i : wf (tInt i).
 
 (** ** Declarations *)
 
@@ -135,10 +141,6 @@ Notation " Γ ,, d " := (snoc Γ d) (at level 20, d at next level).
 
 (** *** Environments *)
 
-Inductive universes :=
-  | Monomorphic (uctx : universe_context)
-  | Polymorphic (uctx : universe_context)
-
 (** See [one_inductive_body] from [declarations.ml]. *)
 Record one_inductive_body := {
   ind_name : ident;
@@ -154,7 +156,7 @@ Record mutual_inductive_body := {
   ind_npars : nat;
   ind_params : context;
   ind_bodies : list one_inductive_body ;
-  ind_universes : universes;
+  ind_universes : universe_context;
   ind_variance : option (list Variance.t);
  }.
 
@@ -192,8 +194,8 @@ Definition program : Type := global_declarations * term.
 (** *** Constant and axiom entries *)
 
 Inductive universes_entry :=
-  | Monomorphic_entry (uctx : universe_context)
-  | Polymorphic_entry (uctx : universe_context)
+  | Monomorphic_entry (uctx : UContext.t)
+  | Polymorphic_entry (uctx : UContext.t).
 
 Record parameter_entry := {
   parameter_entry_type      : term;
